More notes

iris-exercises.v
@@ -6,10 +6,163 @@ From iris.heap_lang.lib Require Import par.
 From iris.base_logic Require Import cancelable_invariants.
 From iris.prelude Require Import options.
 
+From iris.algebra Require Import numbers excl auth gset frac.
+
+Section abql_code.
+
+  (* The ABQL is a variant of a ticket lock which uses an array.
+
+     The lock consists of three things:
+     - An array of booleans which contains true at a single index and false at
+       all other indices.
+     - A natural number, which represents the next available ticket. Tickets are
+       increasing and the remainder from dividing the ticket with the length of
+       the array gives an index in the array to which the ticket corresponds.
+     - The length of the array. The lock can handle at most this many
+       simultaneous attempts to acquire the lock. We call this the capacity of
+       the lock. *)
+  Definition newlock : val :=
+    λ: "cap", let: "array" := AllocN "cap" #false in
+              ("array" +ₗ #0%nat) <- #true ;; ("array", ref #0, "cap").
+
+  (* wait_loop is called by acquire with a ticket. As mentioned, the ticket
+     corresponds to an index in the array. If the array contains true at that
+     index we may acquire the lock otherwise we spin. *)
+  Definition wait_loop : val :=
+    rec: "spin" "lock" "ticket" :=
+      let: "array" := Fst (Fst "lock") in (* Get the first element of the triple *)
+      let: "idx" := "ticket" `rem` (Snd "lock") in (* Snd "Lock" gets the third element of the triple *)
+      if: ! ("array" +ₗ "idx") then #() else ("spin" "lock" "ticket").
+
+  (* To acquire the lock we first take the next ticket using FAA. The wait_loop
+     function then spins until the ticket grants access to the lock. *)
+  Definition acquire : val :=
+    λ: "lock", let: "next" := Snd (Fst "lock") in
+               let: "ticket" := FAA "next" #1%nat in
+               wait_loop "lock" "ticket" ;;
+               "ticket".
+
+  (* To release the lock, the index in the array corresponding to the current
+     ticket is set to false and the next index (possibly wrapping around the end
+     of the array) is set to true. *)
+  Definition release : val :=
+    λ: "lock" "o", let: "array" := Fst (Fst "lock") in
+                   let: "cap" := Snd "lock" in
+                   "array" +ₗ ("o" `rem` "cap") <- #false ;;
+                   "array" +ₗ (("o" + #1) `rem` "cap") <- #true.
+
+End abql_code.
+
+Module spec.
+
+  (* Acquiring the lock consists of taking a ticket and spinning on an entry in
+     the array. If there are more threads waiting to acquire the lock than there
+     are entries in the array, several threads will spin on the same entry in
+     the array, and they may both enter their critical section when this entry
+     becomes true. Thus, to ensure safety the specification must ensure that
+     this can't happen. To this end the specification is that of a ticket lock,
+     but extended with _invitations_.
+
+     Invitations are non-duplicable tokens which gives permission to acquire the
+     lock. In newlock, when a lock is created with capacity `n` the same amount
+     of invitations are created. These are tied to the lock through the ghost
+     name γ. acquire_spec consumes one invitaiton and release_spec hands back
+     one invitation. Together this ensures that at most `n` threads may
+     simultaneously attempt to acquire the lock.
+
+     invitation_split allows the client to split and combine invitations. *)
+
+  Structure abql_spec Σ `{!heapGS Σ} := abql {
+    (* Operations *)
+    newlock : val;
+    acquire : val;
+    release : val;
+    (* Predicates *)
+    is_lock (γ ι κ : gname) (lock : val) (cap : nat) (R : iProp Σ) : iProp Σ;
+    locked (γ κ: gname) (o : nat) : iProp Σ;
+    invitation (ι : gname) (n : nat) (cap : nat) : iProp Σ;
+    (* General properties of the predicates *)
+    is_lock_persistent γ ι κ lock cap R : Persistent (is_lock γ ι κ lock cap R);
+    locked_timeless γ κ o : Timeless (locked γ κ o);
+    locked_exclusive γ κ o o' : locked γ κ o -∗ locked γ κ o' -∗ False;
+    invitation_split γ (n m cap : nat) :
+      invitation γ (n + m) cap ⊣⊢ invitation γ n cap ∗ invitation γ m cap;
+    (* Program specs *)
+    newlock_spec (R : iProp Σ) (cap : nat) :
+      {{{ R ∗ ⌜0 < cap⌝ }}}
+        newlock (#cap)
+      {{{ lk γ ι κ, RET lk; (is_lock γ ι κ lk cap R) ∗ invitation ι cap cap }}};
+    acquire_spec γ ι κ lk cap R :
+      {{{ is_lock γ ι κ lk cap R ∗ invitation ι 1 cap}}}
+        acquire lk
+      {{{ t, RET #t; locked γ κ t ∗ R }}};
+    release_spec γ ι κ lk cap o R :
+      {{{ is_lock γ ι κ lk cap R ∗ locked γ κ o ∗ R }}}
+        release lk #o
+      {{{ RET #(); invitation ι 1 cap }}};
+  }.
+
+End spec.
+
+Section algebra.
+
+  (* We create a resource algebra used to represent invitations. The RA can be
+     thought of as "addition with an upper bound". The carrier of the resource
+     algebra is pairs of natural numbers. The first number represents how many
+     invitations we have and the second how many invitations exists in total.
+
+     We want (a, n) ⋅ (b, n) to be equal to (a + b, n). We never combine
+     elements (a, n) ⋅ (b, m) where n ≠ m. Hence what happens it that case is
+     arbitary, as long the laws for a RA are satisfied. We can not, for instance,
+     just disregard the second upper bound as that whould violate commutativity,
+     and using `max` would not satisfy the laws for validity. We could use
+     agreement, but choose to use `min` instead as it is easier to work with. *)
+  Record addb : Type := Addb { addb_proj : nat * min_nat }.
+
+  Canonical Structure sumRAC := leibnizO addb.
+
+  Local Instance addb_op : Op addb := λ a b, Addb (addb_proj a ⋅ addb_proj b).
+
+  (* The definition of validity matches the intuition that if there exists n
+     invitations in totoal then one can at most have n invitations. *)
+  Local Instance addb_valid : Valid addb :=
+    λ a, match a with Addb (x, MinNat n) => x ≤ n end.
+
+  (* Invitations should not be duplicable. *)
+  Local Instance addb_pcore : PCore addb := λ _, None.
+
+  (* We need these auxiliary lemmas in the proof below. *)
+  Lemma sumRA_op_second a b (n : min_nat) : Addb (a, n) ⋅ Addb (b, n) = Addb (a + b, n).
+  Proof. by rewrite /op /addb_op -pair_op idemp_L. Qed.
+
+  (* If (a, n) is valid ghost state then we can conclude that a ≤ n *)
+  Lemma sumRA_valid a n : ✓(Addb (a, n)) ↔ a ≤ min_nat_car n.
+  Proof. destruct n. split; auto. Qed.
+
+  Definition sumRA_mixin : RAMixin addb.
+  Proof.
+    split; try apply _; try done.
+    - intros ???. rewrite /op /addb_op /=. apply f_equal, assoc, _.
+    - intros ??. rewrite /op /addb_op /=. apply f_equal, comm, _.
+    - intros [[?[?]]] [[?[?]]]. rewrite 2!sumRA_valid nat_op /=. lia.
+  Qed.
+
+  Canonical Structure sumRA := discreteR addb sumRA_mixin.
+
+  Global Instance sumRA_cmra_discrete : CmraDiscrete sumRA.
+  Proof. apply discrete_cmra_discrete. Qed.
+
+  Class sumG Σ := SumG { sum_inG :: inG Σ sumRA }.
+  Definition sumΣ : gFunctors := #[GFunctor sumRA].
+
+  Global Instance subG_sumΣ {Σ} : subG sumΣ Σ → sumG Σ.
+  Proof. solve_inG. Qed.
+
+End algebra.
 
 Section s.
 
-  Context `{!heapGS Σ}.
+  Context `{!heapGS Σ, !spawnG Σ}.
   Notation iProp := (iProp Σ).
 
   Lemma ex_4_2 :
@@ -46,7 +199,6 @@ Section s.
     wp_apply (Spec with "H1") as (r) "H3".
     wp_pure.
     wp_pure.
-    iModIntro.
     iApply "H2".
     done.
   Qed.
@@ -56,9 +208,8 @@ Section s.
       {{{ P ∗ ⌜v = #true⌝ }}} e1 {{{ r, RET r; Q }}} ->
       {{{ P ∗ ⌜v = #true⌝ }}} (if: v then e1 else e2)%E {{{ r, RET r; Q }}}.
   Proof using.
-    iIntros (P Q v e1 e2 Spec H2) "[H4 H5] H6".
-    iDestruct "H5" as "%H3".
-    rewrite H3.
+    iIntros (P Q v e1 e2 Spec H2) "[H4 %H5] H6".
+    subst v.
     wp_if.
     wp_apply (Spec with "[H4]").
     1: iSplit.
@@ -72,8 +223,6 @@ Section s.
     |nil => ⌜l = (InjLV #())⌝
     |cons x tl  => ∃ (hd : loc) l', ⌜l = InjRV #hd⌝ ∗ hd ↦ (#x, l') ∗ ▷ isList l' tl
   end.
-
-  Locate expr.
 
   Definition inc : val :=
     rec: "inc" "x":=
@@ -100,24 +249,138 @@ Section s.
       iDestruct "H1" as "%Heq".
       rewrite Heq.
       wp_match.
-      iModIntro. iApply "H2".
+      iApply "H2".
       done.
-    - iDestruct "H1" as "[%hd [%tl [H1 [H3 H4]]]]".
-      iDestruct "H1" as "%Heq".
-      rewrite Heq.
+    - iDestruct "H1" as "[%hd [%tl [%H1 [H3 H4]]]]".
+      rewrite H1.
       wp_match.
       wp_load.
       wp_pures.
       wp_load.
       wp_pures.
       wp_store.
-      iApply ("Ih" with "[H4]").
-      + Unshelve. 2: apply xs. iApply "H4".
-      + iSimpl in "H2".
-        iNext.
-        iIntros "H4".
-        iApply "H2".
-        iFrame.
-        done.
+      iApply ("Ih" with "H4").
+      iNext.
+      iIntros "H4".
+      iApply "H2".
+      iFrame.
+      done.
   Qed.
+
+  Definition append : val :=
+    rec: "append" "l" "l'" :=
+      match: "l" with
+      InjL "()" => "l'"
+      |InjR "x2" =>
+         let: "p" := !"x2" in
+         let: "r" := "append" (Snd "p") "l'" in
+         "x2" <- (Fst "p", "r");;
+         InjR ("x2") end.
+
+  Lemma append_sepc :
+    forall xs ys l l',
+    {{{ isList l xs ∗ isList l' ys }}}
+      append l l'
+      {{{ r, RET r; isList r (xs ++ ys) }}}.
+  Proof using.
+    iIntros (xs ys l l' ϕ) "[P1 P2] Q".
+    iLöb as "Ih" forall (l xs ϕ).
+    wp_lam.
+    destruct xs as [|h xs'].
+    1: iDestruct "P1" as "%Heq".
+    2: iDestruct "P1" as "[%hd [%tl [%Heq [H3 H4]]]]".
+    all: rewrite Heq;
+      wp_pures.
+    2:
+      wp_load;
+    wp_pures;
+    wp_bind (append tl l');
+    wp_apply ("Ih" with "H4 P2");
+    iIntros (r) "H1";
+    wp_pures;
+    wp_store;
+    wp_pures.
+    all:
+      iApply "Q";
+      iFrame;
+      done.
+  Qed.
+
+  Definition incl : val := λ: "x", ("x" <- !"x" + #1).
+
+  Local Set Default Proof Using "Type*".
+
+  Lemma ex_8_1 :
+    forall l1 (v1 : Z) l2 (v2 : Z),
+      {{{ l1 ↦ #v1 ∗ l2 ↦ #v2 }}}
+        (incl #l1) ||| (incl #l2)
+      {{{ RET (#(), #()); l1 ↦ #(v1 + 1) ∗ l2 ↦ #(v2 + 1) }}}.
+  Proof.
+    iIntros (l1 v1 l2 v2 ϕ) "[H1 H2] Q".
+    unfold incl.
+    wp_smart_apply (wp_par with "[H1] [H2]").
+    + wp_lam. wp_load. wp_store.
+      Unshelve.
+      2: apply (fun v => ⌜v = #()⌝ ∗ l1 ↦ #(v1 + 1))%I.
+      2: apply (fun v => ⌜v = #()⌝ ∗ l2 ↦ #(v2 + 1))%I.
+      iModIntro. iSplit;  done.
+    + wp_lam. wp_load. wp_store. iModIntro. iSplit; done.
+    + iIntros (r1 r2) "[[%Heq1 H1] [%Heq2 H2]]".
+      subst.
+      iApply "Q".
+      iNext. iFrame.
+  Qed.
+
+  Definition linv (l : loc) (n : Z) : iProp := ∃ (m : Z), l ↦ #m ∗ ⌜m >= n⌝%Z.
+
+  Lemma inc_inv :
+    forall l n,
+      inv nroot (linv l n) -∗
+      WP incl #l {{ v, ⌜v = #()⌝ }}.
+    iIntros (l n) "#I".
+    wp_lam.
+    wp_bind (!_)%E.
+    iInv "I" as (m) "[H1 #H2]" "Hclose".
+    wp_load.
+    iMod ("Hclose" with "[H1]") as "_".
+    { iExists m. iSplit; done. }
+    iModIntro.
+    wp_pures.
+    iInv "I" as (m') "[H1 _]" "Hclose".
+    wp_store.
+    iMod ("Hclose" with "[H1]") as "_".
+    { iExists (m + 1)%Z. iNext. iSplit.
+      + done.
+      + iDestruct "H2" as "%H2".
+        iPureIntro. lia. }
+    iModIntro.
+    done.
+  Qed.
+
+  Lemma ex_8_5 :
+    forall l (n : Z),
+      {{{ l ↦ #n }}}
+        (incl #l ||| incl #l);; !#l
+      {{{ v, RET v; ∃ (m : Z), ⌜#m = v⌝ ∗ ⌜m >= n⌝%Z }}}.
+  Proof.
+    iIntros (l n ϕ) "I H1".
+    iMod (inv_alloc nroot _ (linv l n) with "[I]") as "#I".
+    { iExists n. iFrame. iPureIntro. lia. }
+    wp_pures.
+    wp_apply wp_par as (v1 v2) "_".
+    Unshelve.
+    4, 5: apply (fun v => ⌜v = #()⌝)%I.
+    1, 2: iApply inc_inv; iApply "I".
+    iNext.
+    wp_pures.
+    iInv "I" as (m) "[H2 H3]" "Hclose".
+    wp_load.
+    iDestruct "H3" as "%H3".
+    iApply "H1".
+    iExists m.
+    iMod ("Hclose" with "[H2]") as "_".
+    { iExists m. iFrame. done. }
+    done.
+  Qed.
+
 End s.
